Weidenbach_Book/IsaSAT_Backtrack.thy
@@ -451,7 +451,7 @@ definition (in isasat_input_ops) extract_shorter_conflict_list_heur_st
   :: \<open>twl_st_wl_heur \<Rightarrow> (twl_st_wl_heur \<times> nat \<times> nat clause_l) nres\<close>
 where
   \<open>extract_shorter_conflict_list_heur_st = (\<lambda>(M, N, D, Q', W', vm, \<phi>, clvls, cach, lbd, outl,
-       stats). do {
+       stats, ccont, vdom). do {
      ASSERT(M \<noteq> []);
      let K = lit_of (hd M);
      ASSERT(-K \<in># \<L>\<^sub>a\<^sub>l\<^sub>l);
@@ -464,7 +464,7 @@ where
      let cach = empty_cach cach;
      ASSERT(empty_conflict_and_extract_clause_pre ((M, D), outl));
      (D, C, n) \<leftarrow> empty_conflict_and_extract_clause M D outl;
-     RETURN ((M, N, D, Q', W', vm, \<phi>, clvls, cach, lbd, take 1 outl, stats), n, C)
+     RETURN ((M, N, D, Q', W', vm, \<phi>, clvls, cach, lbd, take 1 outl, stats, ccont, vdom), n, C)
   })\<close>
 
 lemma the_option_lookup_clause_assn[sepref_fr_rules]:
@@ -704,7 +704,7 @@ abbreviation (in -)ema_update_fast where
 definition (in isasat_input_ops) propagate_bt_wl_D_heur
   :: \<open>nat literal \<Rightarrow> nat clause_l \<Rightarrow> twl_st_wl_heur \<Rightarrow> twl_st_wl_heur nres\<close> where
   \<open>propagate_bt_wl_D_heur = (\<lambda>L C (M, N, D, Q, W, vm, \<phi>, _, cach, lbd, outl, stats, fema, sema,
-         ccount). do {
+         ccount, vdom). do {
       ASSERT(phase_saving \<phi> \<and> vm \<in> vmtf M \<and> undefined_lit M (-L) \<and> L \<in># \<L>\<^sub>a\<^sub>l\<^sub>l \<and>
          nat_of_lit (C!1) < length W \<and> nat_of_lit (-L) < length W);
       ASSERT(length C > 1);
@@ -722,7 +722,7 @@ definition (in isasat_input_ops) propagate_bt_wl_D_heur
       lbd \<leftarrow> lbd_empty lbd;
       RETURN (Propagated (- L) i # M, N, D, {#L#}, W, vm, \<phi>, zero_uint32_nat,
          cach, lbd, outl, stats, ema_update_fast fema glue, ema_update_slow sema glue,
-          ccount + one_uint32)
+          ccount + one_uint32, vdom @ [nat_of_uint32_conv i])
     })\<close>
 
 definition (in -) lit_of_hd_trail_st_heur :: \<open>twl_st_wl_heur \<Rightarrow> nat literal\<close> where
@@ -737,14 +737,14 @@ definition (in isasat_input_ops) propagate_unit_bt_wl_D_int
   :: \<open>nat literal \<Rightarrow> twl_st_wl_heur \<Rightarrow> twl_st_wl_heur nres\<close>
 where
   \<open>propagate_unit_bt_wl_D_int = (\<lambda>L (M, N, D, Q, W, vm, \<phi>, clvls, cach, lbd, outl, stats,
-      fema, sema, ccount). do {
+      fema, sema, ccount, vdom). do {
       ASSERT(undefined_lit M L \<and> L \<in># \<L>\<^sub>a\<^sub>l\<^sub>l \<and> vm \<in> vmtf M);
       vm \<leftarrow> flush M vm;
       glue \<leftarrow> get_LBD lbd;
       lbd \<leftarrow> lbd_empty lbd;
       RETURN (Propagated (- L) 0 # M, N, D, {#L#}, W, vm, \<phi>, clvls, cach, lbd, outl, stats,
          ema_update_fast fema glue, ema_update_slow sema glue,
-        ccount + one_uint32)})\<close>
+        ccount + one_uint32, vdom)})\<close>
 
 
 definition (in isasat_input_ops) backtrack_wl_D_nlit_heur
@@ -808,7 +808,8 @@ begin
 
 definition (in isasat_input_ops) twl_st_heur_bt :: \<open>(twl_st_wl_heur \<times> nat twl_st_wl) set\<close> where
 \<open>twl_st_heur_bt =
-  {((M', N', D', Q', W', vm, \<phi>, clvls, cach, lbd, outl, stats), (M, N, D, NE, UE, Q, W)).
+  {((M', N', D', Q', W', vm, \<phi>, clvls, cach, lbd, outl, stats, _, _, _, vdom),
+     (M, N, D, NE, UE, Q, W)).
     M = M' \<and> N' = N \<and>
     D' = None \<and>
     Q' = Q \<and>
@@ -818,7 +819,8 @@ definition (in isasat_input_ops) twl_st_heur_bt :: \<open>(twl_st_wl_heur \<time
     no_dup M \<and>
     clvls \<in> counts_maximum_level M D' \<and>
     cach_refinement_empty cach \<and>
-    out_learned M D' outl
+    out_learned M D' outl \<and>
+    dom_m N \<subseteq># mset vdom
   }\<close>
 
 lemma (in isasat_input_ops) twl_st_heur_bt_get_clauses_wl:
@@ -885,8 +887,8 @@ proof -
     obtain M N D NE UE Q W where
       S: \<open>S = (M, N, D, NE, UE, Q, W)\<close>
       by (cases S)
-    obtain W' vm \<phi> clvls cach lbd outl stats where
-      S': \<open>S' = (M, N, D, Q, W', vm, \<phi>, clvls, cach, lbd, outl, stats)\<close>
+    obtain W' vm \<phi> clvls cach lbd outl stats cc cc2 cc3 vdom where
+      S': \<open>S' = (M, N, D, Q, W', vm, \<phi>, clvls, cach, lbd, outl, stats, cc, cc2, cc3, vdom)\<close>
       using S'_S by (cases S') (auto simp: twl_st_heur_def S)
     have
       \<open>(W', W) \<in> \<langle>Id\<rangle>map_fun_rel D\<^sub>0\<close> and
@@ -895,7 +897,8 @@ proof -
       \<open>no_dup M\<close> and
       \<open>clvls \<in> counts_maximum_level M D\<close> and
       cach_empty: \<open>cach_refinement_empty cach\<close> and
-      outl: \<open>out_learned M D outl\<close>
+      outl: \<open>out_learned M D outl\<close> and
+      \<open>dom_m N \<subseteq># mset vdom\<close>
       using S'_S unfolding S S'
       by (auto simp: twl_st_heur_def S)
     obtain T U where
@@ -1055,7 +1058,7 @@ proof -
                    (1 < length C \<longrightarrow> n = get_level M (C ! 1)) \<and>
                    (length C = 1 \<longrightarrow> n = 0)}.
               {((M, N, a, Q, W', vm, \<phi>, clvls, empty_cach cach', lbd, take 1 outl',
-                 stats),
+                   stats, cc, cc2, cc3, vdom),
                 n, C)})
       \<le> \<Down> ?shorter
           (SPEC (\<lambda>S. \<exists>D'. D' \<subseteq># the D \<and>
@@ -1083,7 +1086,8 @@ proof -
         have
           \<open>mset c = mset outl'\<close> and
           \<open>c ! 0 = outl' ! 0\<close> and
-          S': \<open>S' = (M, N, None, Q, W', vm, \<phi>, clvls, empty_cach cach', lbd, take 1 outl', stats)\<close> and
+          S': \<open>S' = (M, N, None, Q, W', vm, \<phi>, clvls, empty_cach cach', lbd, take 1 outl',  
+            stats, cc, cc2, cc3, vdom)\<close> and
           C: \<open>1 < length c \<longrightarrow> highest_lit M (mset (tl c))
                 (Some (c ! 1, get_level M (c ! 1)))\<close>
             \<open>length c = 1 \<longrightarrow> n = 0\<close>
@@ -1126,7 +1130,7 @@ proof -
           using \<open>(W', W) \<in> \<langle>Id\<rangle>map_fun_rel D\<^sub>0\<close> \<open>vm \<in> vmtf M\<close>
             \<open>phase_saving \<phi>\<close>
             \<open>no_dup M\<close>
-            \<open>cach_refinement_empty cach\<close> \<open>c \<noteq> []\<close> \<open>outl' \<noteq> []\<close>
+            \<open>cach_refinement_empty cach\<close> \<open>c \<noteq> []\<close> \<open>outl' \<noteq> []\<close> \<open>dom_m N \<subseteq># mset vdom\<close>
           by (auto simp: twl_st_heur_def S' del_conflict_wl_def
               empty_cach_def cach_refinement_empty_def out_learned_def)
         moreover have \<open>Suc 0 < length c \<Longrightarrow>
@@ -1448,8 +1452,9 @@ proof -
       using \<open>(TnC, T') \<in> ?shorter S'\<close> \<open>1 < length C\<close> find_decomp
       apply (cases U')
       by (auto simp: find_lit_of_max_level_wl_def T')
-    obtain vm' W' \<phi> clvls cach lbd outl stats fema sema ccount where
-        U: \<open>U = (M1, N, None, Q, W', vm', \<phi>, clvls, cach, lbd, outl, stats, fema, sema, ccount)\<close> and
+    obtain vm' W' \<phi> clvls cach lbd outl stats fema sema ccount vdom where
+        U: \<open>U = (M1, N, None, Q, W', vm', \<phi>, clvls, cach, lbd, outl, stats, fema, sema, ccount,
+           vdom)\<close> and
         vm': \<open>vm' \<in> vmtf M1\<close> and
         \<phi>: \<open>phase_saving \<phi>\<close>
       using UU' find_decomp by (cases U) (auto simp: U' T' twl_st_heur_bt_def)
@@ -1460,7 +1465,8 @@ proof -
       n_d_M1: \<open>no_dup M1\<close> and
       empty_cach: \<open>cach_refinement_empty cach\<close> and
       \<open>length outl = Suc 0\<close> and
-      outl: \<open>out_learned M1 None outl\<close>
+      outl: \<open>out_learned M1 None outl\<close>and
+      vdom: \<open>dom_m N \<subseteq># mset vdom\<close>
       using UU' by (auto simp: out_learned_def twl_st_heur_bt_def U U')
     have [simp]: \<open>get_trail_wl_heur S = M\<close> \<open>C ! 1 = L'\<close> \<open>C ! 0 = - lit_of (hd M)\<close> and
       n_d: \<open>no_dup M\<close>
@@ -1492,13 +1498,13 @@ proof -
       using W'W unfolding map_fun_rel_def by (auto simp: image_image)
     then show ?thesis
       supply [[goals_limit=1]]
-      using empty_cach n_d_M1 C_L' W'W outl vmtf undef \<open>1 < length C\<close> uM_\<L>\<^sub>a\<^sub>l\<^sub>l unfolding U U' H
+      using empty_cach n_d_M1 C_L' W'W outl vmtf undef \<open>1 < length C\<close> uM_\<L>\<^sub>a\<^sub>l\<^sub>l vdom unfolding U U' H
         propagate_bt_wl_D_heur_def propagate_bt_wl_D_def set_LBD_def Let_def rescore_clause_def
       by (auto simp: propagate_bt_wl_D_heur_def twl_st_heur_def lit_of_hd_trail_st_heur_def
           propagate_bt_wl_D_def Let_def T' U' U rescore_clause_def S' map_fun_rel_def
           list_of_mset2_def flush_def RES_RES2_RETURN_RES RES_RETURN_RES \<phi> uminus_\<A>\<^sub>i\<^sub>n_iff
           fm_add_new_def get_fresh_index_def RES_RETURN_RES2 RES_RES_RETURN_RES2
-          RES_RES_RETURN_RES lbd_empty_def get_LBD_def set_LBD_def H
+          RES_RES_RETURN_RES lbd_empty_def get_LBD_def set_LBD_def H nat_of_uint32_conv_def
           intro!: ASSERT_refine_left RES_refine exI[of _ C]
           intro!: vmtf_consD)
   qed
@@ -1562,8 +1568,9 @@ proof -
       using \<open>(TnC, T') \<in> ?shorter S'\<close> find_decomp
       apply (cases U')
       by (auto simp: find_lit_of_max_level_wl_def T')
-    obtain vm' W' \<phi> clvls cach lbd outl stats fema sema ccount where
-        U: \<open>U = (M1, N, None, Q, W', vm', \<phi>, clvls, cach, lbd, outl, stats, fema, sema, ccount)\<close> and
+    obtain vm' W' \<phi> clvls cach lbd outl stats fema sema ccount vdom where
+        U: \<open>U = (M1, N, None, Q, W', vm', \<phi>, clvls, cach, lbd, outl, stats, fema, sema, ccount,
+           vdom)\<close> and
         vm': \<open>vm' \<in> vmtf M1\<close>
       using UU' find_decomp by (cases U) (auto simp: U' T' twl_st_heur_bt_def)
     have
@@ -1573,7 +1580,8 @@ proof -
       n_d_M1: \<open>no_dup M1\<close> and
       empty_cach: \<open>cach_refinement_empty cach\<close> and
       \<open>length outl = Suc 0\<close> and
-      outl: \<open>out_learned M1 None outl\<close>
+      outl: \<open>out_learned M1 None outl\<close> and
+      vdom: \<open>dom_m N \<subseteq># mset vdom\<close>
       using UU' by (auto simp: out_learned_def twl_st_heur_bt_def U U')
     have [simp]: \<open>get_trail_wl_heur S = M\<close> \<open>C ! 0 = - lit_of (hd M)\<close> and
       n_d: \<open>no_dup M\<close>
@@ -1586,7 +1594,7 @@ proof -
       using \<open>C \<noteq> []\<close> \<open>C ! 0 = - lit_of (hd M)\<close> \<open>\<not>1 < length C\<close>
       by (cases C) (auto simp del: \<open>C ! 0 = - lit_of (hd M)\<close>)
     show ?thesis
-      using empty_cach n_d_M1  W'W outl vmtf C \<phi> undef uL_M unfolding U U'
+      using empty_cach n_d_M1  W'W outl vmtf C \<phi> undef uL_M vdom unfolding U U'
       by (auto simp: propagate_unit_bt_wl_D_int_def
           propagate_unit_bt_wl_D_def U U' lit_of_hd_trail_st_heur_def
           single_of_mset_def flush_def twl_st_heur_def lbd_empty_def get_LBD_def
@@ -1715,7 +1723,7 @@ sepref_thm propagate_bt_wl_D_code
   rescore_clause_def[simp] flush_def[simp]
   unfolding propagate_bt_wl_D_heur_def isasat_assn_def cons_trail_Propagated_def[symmetric]
   unfolding delete_index_and_swap_update_def[symmetric] append_update_def[symmetric]
-    append_ll_def[symmetric] append_ll_def[symmetric]
+    append_ll_def[symmetric] append_ll_def[symmetric] nat_of_uint32_conv_def
     cons_trail_Propagated_def[symmetric] PR_CONST_def
   apply (rewrite at \<open>(_, add_mset _ \<hole>, _)\<close> lms_fold_custom_empty)+
   by sepref
