Weidenbach_Book/IsaSAT_Propagate_Conflict.thy
@@ -686,7 +686,8 @@ where
      Id \<times>\<^sub>r
      Id \<times>\<^sub>r
      Id \<times>\<^sub>r
-     Id\<close>
+     Id \<times>\<^sub>r
+     \<langle>Id\<rangle>list_rel\<close>
 
 definition (in isasat_input_ops) twl_st_heur_W_list_assn
   :: \<open>twl_st_wl_heur_W_list \<Rightarrow> twl_st_wll_trail \<Rightarrow> assn\<close>
@@ -697,7 +698,8 @@ where
   (list_assn unat_lit_assn) *a
   arrayO_assn (arl_assn nat_assn) *a
   vmtf_remove_conc *a phase_saver_conc *a uint32_nat_assn *a cach_refinement_assn *a
-  lbd_assn *a out_learned_assn *a stats_assn *a ema_assn *a ema_assn *a conflict_count_assn
+  lbd_assn *a out_learned_assn *a stats_assn *a ema_assn *a ema_assn *a
+  conflict_count_assn *a vdom_assn
 \<close>
 
 lemma (in isasat_input_ops) isasat_assn_W_list:
@@ -715,7 +717,8 @@ where
   (list_assn unat_lit_assn) *a
   arrayO_assn (arl_assn uint32_nat_assn) *a
   vmtf_remove_conc *a phase_saver_conc *a uint32_nat_assn *a cach_refinement_assn *a
-  lbd_assn *a out_learned_assn *a stats_assn *a ema_assn *a ema_assn *a conflict_count_assn
+  lbd_assn *a out_learned_assn *a stats_assn *a ema_assn *a ema_assn *a
+  conflict_count_assn *a vdom_assn
 \<close>
 
 lemma (in isasat_input_ops) isasat_fast_assn_W_list:
